\documentclass{article}
\usepackage{xeCJK,amsmath,geometry,float,graphicx,amssymb,zhnumber,booktabs,setspace,tasks,verbatim,amsthm,amsfonts,mathdots}
\usepackage{listings,xcolor,diagbox}
\usepackage{unicode-math}
\geometry{a4paper,scale=0.8}  
\renewcommand\arraystretch{2}
\title{概统作业 (Week 10)}
\author{PB20000113孔浩宇}
\begin{document}
\maketitle
\section{}  %1
\begin{enumerate}
    \item [(0)]选$D$.
    \item [(1)]
    \[
        E(Y_1) 
        = \int_{-\infty}^{+\infty} y \cdot \frac{f_{1} (y)+f_{2} (y)}{2} dy
        = \frac{1}{2}\cdot \left(\int_{-\infty}^{+\infty} y \cdot f_{1} (y) dy + \int_{-\infty}^{+\infty} y \cdot f_{2} (y) dy\right)
        = \frac{E(X_1) + E(X_2)}{2}.
    \]
    \[
        E(Y_2)
        = E\left(\frac{X_1 + X_2}{2}\right)
        = \frac{1}{2}\cdot \left(E(X_1 + X_2)\right)  
        = \frac{E(X_1) + E(X_2)}{2}
        = E(Y_1) .
    \]
    \item [(2)]
    \[
        E(Y_1^2)
        = \int_{-\infty}^{+\infty} y^2 \cdot \frac{f_{1} (y)+f_{2} (y)}{2} dy
        = \frac{1}{2}\cdot \left(\int_{-\infty}^{+\infty} y^2 \cdot f_{1} (y) dy + \int_{-\infty}^{+\infty} y^2 \cdot f_{2} (y) dy\right)
        = \frac{E(X_1^2) + E(X_2^2)}{2}.    
    \]
    \[
        Var(Y_1)
        = E(Y_1^2) - {E(Y_1)}^2   
        = \frac{E(X_1^2) + E(X_2^2)}{2} - {\left(\frac{E(X_1) + E(X_2)}{2}\right)}^2
    \]
    又$Var(X_1) = E(X_1^2) - {E(X_1)}^2,\ Var(X_2) = E(X_2^2) - {E(X_2)}^2$，有
    \[
        Var(Y_1)
        = \frac{Var(X_1) + Var(X_2)}{4} + \frac{E(X_1^2) + E(X_2^2) - 2 E(X_1)E(X_2)}{4}
    \]
    对于$Y_2$，有
    \[
        Var(Y_2)   
        = Var\left(\frac{X_1 + X_2}{2}\right) 
        = \frac{Var(X_1) + Var(X_2)}{4}
    \]
    又由方差$Var(X) = E(X^2) - {E(X)}^2\geq 0$，有
    \[
        \begin{cases}
            \ E(X_1^2) &\geq {E(X_1)}^2 \\ 
            \ E(X_2^2) &\geq {E(X_2)}^2 
        \end{cases}
        \ \Rightarrow\ 
        E(X_1^2) + E(X_2^2) - 2 E(X_1)E(X_2)
        \geq {E(X_1)}^2 + {E(X_2)}^2 - 2 E(X_1)E(X_2)
        \geq 0.
    \]
    故
    \[
        Var(Y_1) - Var(Y_2) \geq 0
        \ \Rightarrow\ 
        Var(Y_1) \geq Var(Y_2).
    \]
\end{enumerate}

\section{(P174 T27)}  %2
\begin{enumerate}
    \item [(1)]
    \[
        P (X=k)    
        = \binom{n}{k} p^{k} {(1-p)}^{n-k} \ (k=0,1,\ldots,n)
    \]
    \[
      M_X (s)
      = E(e^{sX}) 
      = \sum\limits_{k=0}^{n} e^{sk} \binom{n}{k} p^{k} {(1-p)}^{n-k}
      = \sum\limits_{k=0}^{n} \binom{n}{k} {(p e^{s})}^{k} {(1-p)}^{n-k}
      = {(p e^{s} + 1 - p)}^{n}.
    \]
    \item [(2)]
    \[
        P (X=k)
        = \frac{e^{-\lambda} \lambda^{k}}{k!} \ (k=0,1,2,\ldots)    
    \]
    \[
        M_X (s)
        = \sum\limits_{k=0}^{\infty} \frac{e^{-\lambda} \lambda^{k}}{k!} e^{sk}
        = e^{-\lambda} \sum\limits_{k=0}^{\infty} \frac{ {\lambda e^{s}}^{k}}{k!}
        = e^{-\lambda} e^{\lambda e^{s}}    
        = e^{\lambda (e^{s} - 1)} .
    \]
\end{enumerate}

\section{(P175 T30)}  %3
\begin{enumerate}
    \item [(1)]
    \[
        E(X)
        = (0.05 + 0.05 + 0.1) - (0.1 + 0.2 + 0.2)
        = -0.3 .     
    \]
    \[
        E(Y)
        = (0.2 + 0.15 + 0.1) - (0.1 + 0.05 + 0.05)
        = 0.25 .    
    \]
    \[
        E(XY)
        = (0.1 +0.1) - (0.2 + 0.05)
        = -0.05 .    
    \]
    \[
        Cov(X,Y)
        = E(XY) - E(X) E(Y)
        = -0.05 + 0.075
        = 0.025 .
    \]
    \item [(2)]
    \[
        \begin{tabular}{c|cc}
            \diagbox{X}{Y} & 0 & 1 \\
            \hline
            0 & 0.1 & 0.2 \\
            1 & 0.25 & 0.45 
        \end{tabular}
    \]
    \[
        E(X^2)
        = (0.05 + 0.05 + 0.1) + (0.1 + 0.2 + 0.2)    
        = 0.7.
    \]
    \[
        E(Y^2)
        = (0.2 + 0.15 + 0.1) + (0.1 + 0.05 + 0.05)    
        = 0.65
    \]
    \[
        E(X^2 Y^2)
        = 0.45 .  
    \]
    \[
        Cov(X^2 ,Y^2)
        = E(X^2 Y^2) - E(X^2) E(Y^2)
        = 0.45 - 0.7\times 0.65
        = -0.005.
    \]
\end{enumerate}

\section{(P175 T32)}  %4
\begin{enumerate}
    \item [(1)]
    \[
        Cov (\alpha X + \beta Y, \alpha X - \beta Y)
        = \alpha ^2 Var (X) - \beta ^2 Var(Y)
        = (\alpha ^2 - \beta ^2) \sigma^2 .
    \]
    \item [(2)]
    又$(\alpha X + \beta Y, \alpha X - \beta Y)$服从二维正态分布，故
    当$\alpha = \pm \beta $时，$\alpha X + \beta Y, \alpha X - \beta Y$相互独立.
\end{enumerate}

\section{(P175 T34)}  %5
\begin{enumerate}
    \item [(1)]
    \[
        E(X)
        = \iint_{(x,y) \in G} x dx dy
        = 0.   
        \qquad
        E(Y)
        = \iint_{(x,y) \in G} y dx dy
        = 0.   
    \]
    \[
        E(XY)
        = \iint_{(x,y) \in G} xy dx dy
        = 0.   
    \]
    故
    \[
        Cov(X,Y)
        = E(XY) - E(X) E(Y)
        = 0.    
    \]
    \item [(2)]
    \[
        f(x,y) = \frac{1}{S} = \frac{1}{2}.    
    \]
    \[
        f_X (x) 
        = \int_{-\infty}^{+\infty} dy \int_{|x|+|y|\leq 1} f(x,y) dx
        = 
        \begin{cases}
            \ 1+x, & (-1\leq x\leq 0)\\
            \ 1-x, & (0< x \leq 1)    
        \end{cases}
    \]
    \[
        f_Y (y) 
        = \int_{-\infty}^{+\infty} dx \int_{|x|+|y|\leq 1} f(x,y) dy
        = 
        \begin{cases}
            \ 1+y, & (-1\leq y \leq 0)\\
            \ 1-y, & (0< y \leq 1)    
        \end{cases}
    \]
    \[
        f(x,y) \neq f_X (x) f_Y(y)
        \ \Rightarrow\ 
        X,Y \mbox{不相互独立}.    
    \]
\end{enumerate}

\end{document}