\documentclass{article}
\usepackage{xeCJK,amsmath,geometry,float,graphicx,amssymb,zhnumber,booktabs,setspace,tasks,verbatim,amsthm,amsfonts,mathdots}
\usepackage{listings,xcolor,diagbox}
\usepackage{unicode-math}
\geometry{a4paper,scale=0.8}  
\renewcommand\arraystretch{2}
\title{概统作业 (Week 9)}
\author{PB20000113孔浩宇}
\begin{document}
\maketitle
\section{(P173 T16)}  %1
\begin{enumerate}
    \item [(1)]
    \[
        E(sgn (X)) 
        = \int_{-2}^{1} sgn(x)\cdot f(x) dx
        = \frac{1}{3}\cdot \left(\int_{-2}^{0}sgn(x) dx + \int_{0}^{1} sgn(x) dx\right) 
        = \frac{1}{3} \cdot (-1)
        = -\frac{1}{3}.   
    \]
    \[
        E({sgn}^2 (X))
        = \int_{-2}^{1} {sgn}^2 (x) \cdot f(x) dx
        = \frac{1}{3} \cdot \left(\int_{-2}^{0} {sgn}^{2}(x) dx  + \int_{0}^{1} {sgn}^{2} (x) dx \right)
        = \frac{1}{3} \cdot 3
        = 1.
    \]
    因此
    \[
        Var(sgn(X))
        = E({sgn}^2 (X)) - {\left(E(sgn(X))\right)}^2  
        = 1 - \frac{1}{9}
        = \frac{8}{9} 
    \]
    \item [(2)]
    \[
        E(sgn(X) \cdot X)
        = \int_{-\infty}^{+\infty} sgn(x) \cdot x \cdot f(x) dx    
        = 2 \int_{0}^{+\infty} x \cdot \frac{1}{\sqrt{2\pi}} e^{-\frac{x^2}{2}} dx
        = - \sqrt{\frac{2}{\pi}} \cdot e^{-\frac{x^2}{2}} \big| _{0}^{+\infty}
        = \sqrt{\frac{2}{\pi}}.
    \]
\end{enumerate}

\section{(P173 T18)}  %2
\begin{enumerate}
    \item [(1)]
    \[
        \begin{aligned}
        F(y)
        & = P(Y\leq y)\\
        & = P(Y\leq y, X=1) + P(Y\leq y, X=2)\\
        & = P(Y\leq y| X=1) \cdot P(X=1) + P(Y\leq y | X=2) \cdot P(X=2)\\
        & = \frac{1}{2} \left[ P(Y\leq y| X=1) + P(Y\leq y| X=2) \right]
        \end{aligned}
    \]
    \begin{enumerate}
        \item [(a)]$y<0$
        \[
            F(y) = 0.    
        \]
        \item [(b)]$0\leq y <1$
        \[
            F(y) = \frac{1}{2}y + \frac{1}{2}\cdot \frac{y}{2} = \frac{3}{4} y.    
        \]
        \item [(c)]$1\leq y <2$
        \[
            F(y) = \frac{1}{2} + \frac{1}{2}\cdot \frac{y}{2} = \frac{1}{4}y + 2.    
        \]
        \item [(d)]$y\geq 2$
        \[
            F(y) = 1.
        \]
    \end{enumerate}
    故
    \[
        F_{Y} (y)    
        = 
        \begin{cases}
            0,  & (y<0) \\
            \frac{3}{4}y, & (0\leq y <1) \\
            \frac{y}{4} + \frac{1}{2}, & (1\leq y <2) \\
            1. &(y\geq 2) 
        \end{cases}
    \]
    \item [(2)]
    \[
        f_{Y} (y)
        = F_{Y} '(y)
        = 
        \begin{cases}
            \displaystyle{\frac{3}{4}} & (0\leq y <1)\\
            \\
            \displaystyle{\frac{1}{4}} & (1\leq y <2)\\
            \\
            0. & \mbox{其他}
        \end{cases}
    \]
    \[
        E(Y)
        = \int_{-\infty}^{+\infty} y \cdot f_{Y} (y) dy
        = \frac{3}{4} \int_{0}^{1} y dy + \frac{1}{4} \int_{1}^{2} y dy
        = \frac{3}{8} y^2 \big|_{0}^{1} + \frac{1}{8} y^2 \big|_{1}^{2}
        = \frac{3}{4}.
    \]
\end{enumerate}

\section{(P174 T24)}  %3
\begin{enumerate}
    \item [(1)]
    \[
        E(X+Y-3\mu)
        = E(X) + E(Y) - 3\mu
        = \mu + \mu - 3\mu 
        = 0.   
    \]
    \[
        Var(X+Y-3\mu)
        = Var(X) + Var(Y) + 2 Cov(X,Y)
        = \sigma^2 + 2\sigma^2 
        + 2 \cdot \sigma \cdot \sqrt{2}\sigma \cdot \frac{\sqrt{2}}{4}
        = 4\sigma^2 .
    \]
    故
    \[
        X+Y-3\mu \sim N(0 , 4\sigma^2)    
    \]
    记$Z= X+Y-3\mu$，有
    \[
        f_{Z} (z)
        = \frac{1}{2\sqrt{2\pi} \sigma} e^{-\frac{z^2}{8 \sigma^2}}
    \]
    记${(X+Y-3\mu)}_{+} = \max\{ X+Y-3\mu , 0 \} = \max\{ z, 0 \} = g(z)$，有
    \[
        E(g(z))
        = \int_{-\infty}^{+\infty} g(z)\cdot f_{Z} (z) dz
        = \int_{0}^{+\infty} z \cdot \frac{1}{2\sqrt{2\pi} \sigma} e^{-\frac{z^2}{8 \sigma^2}} dz
        = \sqrt{\frac{2}{\pi}} \sigma .
    \]
    \item [(2)]
    \[
        E\left( g^2 (z) \right)  
        = \int_{-\infty}^{+\infty} g^2 (z)\cdot f_{Z} (z) dz
        = \int_{0}^{+\infty} z^2 \cdot \frac{1}{2\sqrt{2\pi} \sigma} e^{-\frac{z^2}{8 \sigma^2}} dz
        = \frac{1}{2} E(z^2)
        = \frac{1}{2} \left[ Var(z) + {(E(z))}^2 \right]
        = 2 \sigma^2 .
    \]
    \[
        Var(g(z)) 
        = E(g^2 (z)) - {\left( E(z) \right)}^2
        = (2-\frac{2}{\pi}) \sigma.
    \]
\end{enumerate}

\section{(P174 T26)}  %4
\begin{enumerate}
    \item [(1)]
    记$\varphi (x_1 , x_2 , x_3) = x_1 + x_2 + x_3$，则
    \[
        E(X_1 + X_2 + X_3)
        = \oiint\limits_{x_1^2 + x_2^2 + x_3^2 = 1} \varphi(x_1 , x_2 , x_3) dS
        = \oiint\limits_{x_1^2 + x_2^2 + x_3^2 = 1} x_1 dS + \oiint\limits_{x_1^2 + x_2^2 + x_3^2} x_2 dS + \oiint\limits_{x_1^2 + x_2^2 + x_3^2} x_3 dS
        = 0.
    \]
    \item [(2)]
    \[
        E\left[ {(X_1 + X_2 + X_3)}^2\right]
        = \oiint\limits_{x_1^2 + x_2^2 + x_3^2 = 1} {(x_1 + x_2 + x_3)}^2 dS
        = \oiint\limits_{x_1^2 + x_2^2 + x_3^2 = 1} 1 + 2 (x_1 x_2 + x_1 x_3 + x_2 x_3) dS
    \]
    又
    \[
        \oiint\limits_{x_1^2 + x_2^2 + x_3^2 = 1} x_1 x_2 dS 
        = \oiint\limits_{x_1^2 + x_2^2 + x_3^2 = 1} x_1 x_3 dS 
        = \oiint\limits_{x_1^2 + x_2^2 + x_3^2 = 1} x_2 x_3 dS
        = 0.
    \]
    \[
        Var(X_1 + X_2 + X_3)
        = E\left[ {(X_1 + X_2 + X_3)}^2\right] - {\left[E(X_1 + X_2 + X_3) \right]}^2 
        = \oiint\limits_{x_1^2 + x_2^2 + x_3^2 = 1} dS
        = 4\pi .
    \]
\end{enumerate}

\section{(P178 T55)}  %5
\begin{proof}
    \begin{enumerate}
        \item []
        \item [(1)]
        \begin{enumerate}
            \item [(a)]证明1：
            \[
                \forall\ X\in [0,1],\ 
                X^2\leq X
                \ \Rightarrow\ 
                Var(X)
                = E(X^2) - {E(X)}^2
                \leq E(X) - {E(X)}^2   
            \]
            记$t = E(X)$，则$0\leq t \leq 1$，有
            \[
                Var(X) = t(1-t) \leq {\left(\frac{t+(1-t)}{2}\right)}^2 = \frac{1}{4}.    
            \]
            \item [(b)]证明2：
            
            取$Y = X - \displaystyle{\frac{1}{2}}$ ，有
            \[
                Var(Y) = Var(X),\ 
                -\frac{1}{2} \leq Y \leq \frac{1}{2}
                \ \Rightarrow\ 
                0\leq Y^2 \leq \frac{1}{4}
                \ \Rightarrow\ 
                E(Y^2) \leq \frac{1}{4}
            \]
            故
            \[
                Var(X) 
                = Var(Y) = E(Y^2) - {\left(E(Y)\right)}^2 
                \leq \frac{1}{4} - {\left(E(Y)\right)}^2 
                \leq \frac{1}{4}
            \]
        \end{enumerate}
        
        当且仅当$E(X)=\frac{1}{2}$且$E(X) = E(X^2)$时等号成立，即$X$服从$P(X=1)=P(X=0)=\displaystyle{\frac{1}{2}}$的分布时.
        \item [(2)]当$0<a\leq X\leq b$时，有$Var(X)\leq \displaystyle{\frac{{(b-a)}^2}{4}}$，当且仅当$X$服从$P(X=a)=P(X=b)=\displaystyle{\frac{1}{2}}$的分布时取等.
        
        取$Y = X - \displaystyle{\frac{a+b}{2}}$ ，有
        \[
            Var(Y) = Var(X), \ 
            \frac{a-b}{2} \leq Y \leq \frac{b-a}{2}
            \ \Rightarrow\ 
            0 \leq Y^2 \leq \frac{{(b-a)}^2}{4}
            \ \Rightarrow\ 
            E(Y^2)\leq \frac{{(b-a)}^2}{4}
        \]
        故
        \[
            Var(X) 
            = Var(Y) = E(Y^2) - {\left(E(Y)\right)}^2 
            \leq \frac{{(b-a)}^2}{4} - {\left(E(Y)\right)}^2 
            \leq \frac{{(b-a)}^2}{4}
        \]
    \end{enumerate}
\end{proof}

\end{document}